src/smtencoding/FStar.SMTEncoding.Term.fsti
@@ -243,6 +243,7 @@ val mkBvMod   : (int -> (term * term) -> Range.range -> term)
 val mkBvMul   : (int -> (term * term) -> Range.range -> term)
 val mkStrLen  : term -> Range.range -> term
 val mkStrCat  : (term * term) -> Range.range -> term
+val mkStrAt   : (term * term) -> Range.range -> term
 
 val mkITE: (term * term * term) -> Range.range -> term
 val mkCases : list term -> Range.range -> term
